done with second admit from aes

src/crypto/aes/GCM_helpers_i.fst
@@ -287,7 +287,33 @@ let pad_to_128_bits_lower (q:quad32) (num_bytes:int) =
     
             
 let pad_to_128_bits_upper (q:quad32) (num_bytes:int) =
-  admit();       ///////////////////////////////  TODO!!!  //////////////////////////////////////////////////////////////
-  ()
-                   
-  
+  let Mkfour x0 x1 x2 x3 = q in
+  let new_hi = (hi64 q) % pow2 ((num_bytes - 8) * 8) in
+  assert_norm (pow2 64 == pow2_64); // refinement on Words_s.pow2_64?
+  assert (new_hi < pow2_64);
+  let q' = insert_nat64 q new_hi 1 in
+  let new_hi_two = Words.Two_s.nat_to_two 32 new_hi in
+  assert_by_tactic (insert_nat64 (Mkfour x0 x1 x2 x3) new_hi 1 == Mkfour x0 x1 new_hi_two.lo new_hi_two.hi)
+    (fun () -> norm[delta]; trefl ());
+
+  assert_norm (hi64 (Mkfour x0 x1 x2 x3) == Words.Two_s.two_to_nat 32 (Mktwo x2 x3));
+  assert (new_hi == (Words.Two_s.two_to_nat_unfold 32 (Mktwo x2 x3)) % pow2 ((num_bytes - 8) * 8));
+  assert (q' == Mkfour x0 x1 new_hi_two.lo new_hi_two.hi); 
+
+  // Easier to prove that le_quad32_to_bytes q' == ... and then derive the goal from injectivity.
+  let q'_bytes = le_quad32_to_bytes q' in
+  FStar.Classical.forall_intro (le_quad32_to_bytes_sel q');
+  FStar.Classical.forall_intro (le_quad32_to_bytes_sel q);
+  assert (q'_bytes == le_quad32_to_bytes (Mkfour x0 x1 new_hi_two.lo new_hi_two.hi));
+  assert (forall i. i <= 8 /\ i < 12 ==> index q'_bytes i == four_select (nat_to_four 8 new_hi_two.lo) (i % 4));
+  assert (forall i. i <= 8 /\ i < 12 ==> index (slice (le_quad32_to_bytes q) 0 num_bytes) i == 
+					     four_select (nat_to_four 8 new_hi_two.lo) (i % 4));
+  assert (forall i. i <= 12 /\ i < 16 ==> index q'_bytes i == four_select (nat_to_four 8 new_hi_two.hi) (i % 4));
+  assert (forall i. i <= 12 /\ i < 16 ==> index (slice (le_quad32_to_bytes q) 0 num_bytes) i == 
+					     four_select (nat_to_four 8 new_hi_two.hi) (i % 4));
+  assert (forall i. i < 4 ==> index q'_bytes i == four_select (nat_to_four 8 x0) (i % 4));
+  assert (forall i. i < 4 ==> index (slice (le_quad32_to_bytes q) 0 num_bytes) i == 
+					     four_select (nat_to_four 8 x0) (i % 4));
+  assert (forall i. i <= 4 /\ i < 8 ==> index q'_bytes i == four_select (nat_to_four 8 x1) (i % 4));
+  assert (forall i. i <= 4 /\ i < 8 ==> index (slice (le_quad32_to_bytes q) 0 num_bytes) i == 
+				     four_select (nat_to_four 8 x1) (i % 4))
